Try alternate formulation of PCM1.  That works.  PCM2 still has issues.

Test/modules/PCM1.dfy
@@ -9,10 +9,10 @@ abstract module PCM {
 }
 module Tokens(pcm: PCM) {
   import opened GhostLoc
-  type {:extern} Token(!new) {
-    function {:extern} loc() : Loc
-    function {:extern} get() : pcm.M
-  }
+  type {:extern} Token(!new)
+
+  function {:extern} loc(t:Token) : Loc
+  function {:extern} get(t:Token) : pcm.M
 }
 abstract module PCMExt(Base: PCM) refines PCM {
   type B = Base.M
@@ -27,6 +27,6 @@ module PCMExtMethods(Base: PCM, Ext: PCMExt(Base)) {
       linear b: BaseTokens.Token,
       ghost f': F)
    : (linear f_out: ExtTokens.Token)
-  ensures f_out.loc().ExtLoc? && f_out.loc().base_loc == b.loc()
-  ensures f_out.get() == f'
+  ensures ExtTokens.loc(f_out).ExtLoc? && ExtTokens.loc(f_out).base_loc == BaseTokens.loc(b)
+  ensures ExtTokens.get(f_out) == f'
 }
